	\section{Numerical scheme}
	\subsection{Macroscopic model}
	
The equations for the macroscopic model can be written as:

\begin{equation}
 \p_t f^{S}=\Linkop(f^S,f^T)+\Difop(f^S)+\Logop(f^S,f^T), \quad S\neq T\in\{A,B\}
\end{equation}
with
\begin{equation}
\Linkop(f^S,f^T)=  \nabla \cdot (f^S\nabla_x(\Phi^{SS}* f^S)) + \nabla \cdot (f^S \nabla_x \Phi^{ST}*f^T)
\end{equation}
\begin{equation}
\Difop(f^S)= D_S \Delta_x f^S
\end{equation}
\begin{equation}
\Logop(f^S,f^T)=\nu^{S}f^S\left( 1-\frac{f^S+f^T}{f^{*}} \right)
\end{equation}


\subsubsection{Spatial Discretization}


First we focus on the spatial discretization of the equations. A general semi-discrete finite-volume scheme can be written as follows:
\begin{equation}
\frac{d f^{S}_{j,k}}{dt}=\Linkop_{j,k}+\Difop_{j,k}+\Logop_{j,k}
\end{equation}
The discrtization of the terms $\Difop_{j,k}$ and $\Logop_{j,k}$ is straightforward and we will present only the details for the link operator $\Linkop_{j,k}$. As in \textbf{citation}, we set :
\begin{equation}
\Linkop_{j,k}= -\frac{F^{x}_{j+\frac{1}{2},k}-F^{x}_{j-\frac{1}{2},k}}{\Delta x}-\frac{F^{y}_{j,k+\frac{1}{2}}-F^{y}_{j,k-\frac{1}{2}}}{\Delta y},
\end{equation}
with
\begin{equation*}
 F^{x}_{j+\frac{1}{2},k}=u^{+}_{j+\frac{1}{2},k}f^{E}_{j,k}-
u^{-}_{j+\frac{1}{2},k}f^{W}_{j+1,k}, \quad F^{y}_{j,k+\frac{1}{2}}=u^{+}_{j,k+\frac{1}{2}}f^{N}_{j,k}-
u^{-}_{j,k+\frac{1}{2}}f^{S}_{j,k+1}
\end{equation*}
% $$F^{x}_{j-\frac{1}{2},k}=u^{+}_{j-\frac{1}{2},k}f^{E}_{j-1,k}-
% u^{-}_{j-\frac{1}{2},k}f^{W}_{j,k}, \quad F^{y}_{j,k-\frac{1}{2}}=u^{+}_{j,k-\frac{1}{2}}f^{N}_{j,k-1}-
% u^{-}_{j,k-\frac{1}{2}}f^{S}_{j,k}$$
where $u^{+}=\max(u,0)$, $u^{-}=-\min(u,0)$ and with 

$$u_{j+\frac{1}{2},k}=-\frac{\xi_{j+1,k}-\xi_{j,k}}{\Delta x}, \quad u_{j,k+\frac{1}{2}}=-\frac{\xi_{j,k+1}-\xi_{j,k}}{\Delta y}$$.

% $$u_{j-\frac{1}{2},k}=-\frac{\xi_{j,k}-\xi_{j-1,k}}{\Delta x}, \quad u_{j,k-\frac{1}{2}}=-\frac{\xi_{j,k}-\xi_{j,k-1}}{\Delta y}$$.

$$ \xi_{j,k}=\Delta x \Delta y \sum_{i,\l} \tilde{\Phi}^{SS}_{j-i,k-\l} f^{S}_{i,\l}+
\tilde{\Phi}^{ST}_{j-i,k-\l} f^{T}_{i,\l} $$
with ${\Phi}^{SS}(x_j-x_i,x_k-x_{\l})$. We compute te convolution term with a FFT method.
% $$ \xi_{j,k}=\Delta x \Delta y \sum_{i} \sum_{\l} \tilde{\Phi}^{AA}(x_{j}-x_{i},x_{k}-x_{\l}) f^{A}_{i,\l}+
% \tilde{\Phi}^{AB}(x_{j}-x_{i},x_{k}-x_{\l}) f^{B}_{i,\l} $$
% 
% $$ F_R=\nu_b^{A}f^{A}_{j,k}\left(1-\frac{f^{A}_{j,k}+f^{B}_{j,k}}{f^{*}}\right). $$


\subsubsection{Time Discretization}

The time discretization of the equations is done with an Euler scheme. The diffusion term is treated implicitly whereas the link term and the logistic term are treated explicitly. This leads to the following scheme:
\begin{equation}
	\frac{f_{j,k}^{S,n+1}-f_{j,k}^{S,n}}{\Delta t}=\Linkop_{j,k}^n+\Difop_{j,k}^{n+1}+\Logop_{j,k}^n
\end{equation}
%  $$(LO)^{n}=-\frac{F^{x,n}_{j+\frac{1}{2},k}-F^{x,n}_{j-\frac{1}{2},k}}{\Delta x}-\frac{F^{y,n}_{j,k+\frac{1}{2}}-F^{y,n}_{j,k-\frac{1}{2}}}{\Delta y}.	$$
\subsection{Microscopic model}
We perform numerical simulations on a $2D$ domain as in [cit] $[-L, L]\times[-L,L]=[-7.5,7.5]^2$ with periodic boundary conditions. We set diffusion constants $D_A=D_B=10^{-4}$ and investigate different values of inter- and intra- species intensities such as $\ka^{AA}, \ka^{BB}, \ka^{AB}=s\tilde{\ka}^{AB},  \ka^{BA}=s\tilde{\ka}^{BA}.$ For each equation of system \eqref{micro} we have the following time discretization:

\begin{equation}
X_i^{n+1}=X_i^{n}-\mu\nabla_{X_i} W(X^n)\Delta t^n+\sqrt{2D \Delta t^n}\mathcal{N}(0,1)
\end{equation}
 $\mathcal{N}(0,1)$ is the normal distribution with mean 0 and standard
deviation 1. \\
By the addition of logistic growth term in the model, the number of particles $N_A, N_B$ changes at each time step. Daughter cells are supposed to born at distance $r$ from 'parent' cells that divide themselves. In our model we set $r=0.5$.

%% R related to link term (repulsion)
%% R0 related to logistic term (distance for birth and death)
%% r related to distance between parents and daughter cells

% logistic term
\begin{equation}
\beta_{A}=b_{0}^{A}-(b_{0}^{A}-\theta_{A})\left(\frac{N_A+N_B}{N^{*}}\right), \quad\quad \delta_{A}=d_{0}^{A}+(\theta_{A}-d_{0}^{A})\left(\frac{N_A+N_B}{N^{*}}\right)
\end{equation}

