\section{Stability analysis}


\begin{equation}
s^{*}_{\nu_b,\nu_d \ne 0}=\frac{(24 D_A+c'^{AA})\nu_{b}^{B}\bar{f}^{B}+(24 D_B+c'^{BB})\nu_{b}^{A}\bar{f}^A}{\nu_{b}^{B}\bar{f}^B\tilde{c}'^{AB}+\nu_{b}^{A}\bar{f}^A\tilde{c}'^{BA}}
\end{equation}

with $\bar{f}^A$ and $\bar{f}^B$ constant steady states, not necessarily equal and 
$c'^{ST}=\frac{2\pi k^{ST} \bfA \nu_c^{ST} R^{4}}{\nu_d^{ST}}$, $S,T \in \{ A,B \}$.

We define $c'^{AA}=k_1 \bfA, c'^{BB}=k_2\bfB, c'^{AB}=k_3\bfA, c'^{BA}=k_4\bfB$.
By $\bar{f}^B=f^*-\bar{f}^A$ we rewrite the following $s^*$:

\begin{equation}
s^{*}_{\nu_b,\nu_d \ne 0}=\frac{(24 D_A+k_1\bfA)\nu_{b}^{B}(f^*-\bfA)+(24 D_B+k_2(f^*-\bfA))\nu_{b}^{A}\bar{f}^A}{\nu_{b}^{B}(f^*-\bfA)k_3\bfA+\nu_{b}^{A}\bar{f}^Ak_4(f^*-\bfA)}
\end{equation}

To simplify notation, we take into account the following function depending on $\bfA$ and its derivative :
$$F(\bfA)=\frac{\a \bfA + \b (\bfA)^2 + \g}{\d \bfA + \eps(\bfA)^2}, \quad\quad 
\frac{\p F(\bfA)}{\p \bfA}=\frac{(\bfA)^2(\b \d-\a \eps)-2\eps \g \bfA - \g\d}{(\d \bfA+\eps (\bfA)^2)^2}$$ 
with parameters 
\begin{equation}
\a= 24D_B \nu_b^A -24 D_A \nu_b^B +k_1 \nu_b^B f^* + k_2 \nu_b^A f^* \quad
\b=-k_1 \nu_b^B -k_2 \nu_b^A \quad
\g= 24 D_A \nu_b^B f^*
\d= k_3\nu_b^B f^*+k_4 \nu_b^A f^*
\end{equation}




